examples/seplogic/SL.Effect.fst
@@ -23,9 +23,9 @@ let st_wp (a:Type) = post a -> pre
 (* unfold *) let id_wp (a:Type) (x:a) (p:post a) (m:memory) = p x emp
 
 (* unfold *)  let st_if_then_else (a:Type) (p:Type) (wp_then:st_wp a) (wp_else:st_wp a) (post:post a) (m0:memory) =
-  // l_ITE p (wp_then post m0) (wp_else post m0)
-  l_ITE p ((bind_wp range_0 a a wp_then (id_wp a)) post m0)
-          ((bind_wp range_0 a a wp_else (id_wp a)) post m0)
+  l_ITE p (wp_then post m0) (wp_else post m0)
+  // l_ITE p ((bind_wp range_0 a a wp_then (id_wp a)) post m0)
+  //         ((bind_wp range_0 a a wp_else (id_wp a)) post m0)
 
 (* unfold *)  let st_ite_wp (a:Type) (wp:st_wp a) (p:post a) (m0:memory) = wp p m0
 
